removed mini_prelude, updated files which dependend on it, adapted basis/translation to deal with new std_prelude

basis/translation/mllistProgScript.sml
@@ -1,11 +1,13 @@
-open preamble ml_translatorLib ml_progLib
-open mllistTheory
+open preamble ml_translatorLib ml_progLib std_preludeTheory 
+open mllistTheory ml_translatorTheory
 
 
 
 (*this library depends on nothing*)
 val _ = new_theory"mllistProg"
-val result = register_type ``:cpn``
+
+val _ = translation_extends "std_prelude"
+
 val _ = ml_prog_update (open_module "List");
 
 
@@ -14,15 +16,19 @@ val _ = ml_prog_update (add_dec ``Dtabbrev ["'a"] "list" (Tapp [Tvar "'a"] (TC_n
 
 val result = translate LENGTH;
 
-
-val result = translate APPEND;
-
-
 val result = translate HD;
+val hd_side_def = Q.prove(
+  `!xs. hd_side xs = ~(xs = [])`,
+  Cases THEN FULL_SIMP_TAC (srw_ss()) [fetch "-" "hd_side_def"])
+  |> update_precondition;
 
 val result = translate tl_def;
 val result = next_ml_names := ["TL_hol"]; 
 val result = translate TL;
+val tl_1_side_def = Q.prove(
+  `!xs. tl_1_side xs = ~(xs = [])`,
+  Cases THEN FULL_SIMP_TAC (srw_ss()) [fetch "-" "tl_1_side_def"])
+  |> update_precondition;
 
 
 val result = translate LAST_DEF;
@@ -32,7 +38,7 @@ val result = translate getItem_def;
 
 
 val result = translate (EL |> REWRITE_RULE[GSYM nth_def]);
-
+val nth_side_def = theorem"nth_side_def";
 
 val result = translate (TAKE_def |> REWRITE_RULE[GSYM take_def]);
 
@@ -40,15 +46,8 @@ val result = translate (TAKE_def |> REWRITE_RULE[GSYM take_def]);
 val result = translate (DROP_def |> REWRITE_RULE[GSYM drop_def]);
 
 
-val result = next_ml_names := ["rev"];
-val result = translate REVERSE_DEF;
-
-
 val result = next_ml_names := ["concat"];
 val result = translate FLAT;
-
-
-val result = translate REV_DEF;
 
 
 val result = translate MAP;
@@ -96,42 +95,22 @@ val result = translate collate_def;
 val result = translate zip_def;
 
 
-(*
-(*these need to be moved elsewhere *)
-val result = translate FST;
-val result = translate SND;
-val result = translate K_DEF;
-val result = translate IN_DEF;
-
-
 (*Extra translations from std_preludeLib.sml *)
+val res = translate LENGTH_AUX_def;
+val res = translate LENGTH_AUX_THM;
 val result = translate SUM;
 val result = translate UNZIP;
 val result = translate PAD_RIGHT;
 val result = translate PAD_LEFT;
-val result = translate MEM;
-(* val result = translate MEMBER_def;  unsure what this is meant to be but I can't find MEMBER_def with DB.find*)
-val result = translate (ALL_DISTANCE |> REWRITE_RULE [MEMBER_INTRO]);
+val result = translate (ALL_DISTINCT |> REWRITE_RULE [MEMBER_INTRO]);
 val result = translate isPREFIX;
 val result = translate FRONT_DEF;
 val result = translate (splitAtPki_def |> REWRITE_RULE [SUC_LEMMA])
 
+
 val front_side_def = Q.prove(
   `!xs. front_side xs = ~(xs = [])`,
   Induct THEN ONCE_REWRITE_TAC [fetch "-" "front_side_def"]
-  THEN FULL_SIMP_TAC (srw_ss()) [CONTAINER_def])
-  |> update_precondition;
-
-val zip_side_def = Q.prove(
-  `!x. zip_side x = (LENGTH (FST x) = LENGTH (SND x))`,
-  Cases THEN Q.SPEC_TAC (`r`,`r`) THEN Induct_on `q` THEN Cases_on `r`
-  THEN ONCE_REWRITE_TAC [fetch "-" "zip_side_def"]
-  THEN FULL_SIMP_TAC (srw_ss()) [])
-  |> update_precondition;
-
-val el_side_def = Q.prove(
-  `!n xs. el_side n xs = (n < LENGTH xs)`,
-  Induct THEN Cases_on `xs` THEN ONCE_REWRITE_TAC [fetch "-" "el_side_def"]
   THEN FULL_SIMP_TAC (srw_ss()) [CONTAINER_def])
   |> update_precondition;
 
@@ -141,6 +120,12 @@ val last_side_def = Q.prove(
   THEN FULL_SIMP_TAC (srw_ss()) [CONTAINER_def])
   |> update_precondition;
 
-*)
+
+val nth_side_def = Q.prove(
+  `!n xs. nth_side xs n = (n < LENGTH xs)`,
+  Induct THEN Cases_on `xs` THEN ONCE_REWRITE_TAC [fetch "-" "nth_side_def"]
+  THEN FULL_SIMP_TAC (srw_ss()) [CONTAINER_def])
+  |> update_precondition;
+
 val _ =  ml_prog_update (close_module NONE);
 val _ = export_theory()
