basis/translation/mlarrayProgScript.sml
@@ -1,0 +1,112 @@
+open preamble
+     ml_translatorTheory ml_translatorLib semanticPrimitivesTheory 
+     cfHeapsTheory cfTheory cfTacticsBaseLib cfTacticsLib ml_progLib mlvectorProgTheory
+
+val _ = new_theory"mlarrayProg"
+
+val _ = translation_extends "mlvectorProg";
+
+
+fun append_prog tm = let
+  val tm = QCONV EVAL tm |> concl |> rand
+  in ml_prog_update (ml_progLib.add_prog tm pick_name) end
+
+fun append_dec tm = let
+  val tm = QCONV EVAL tm |> concl |> rand
+  in ml_prog_update (ml_progLib.add_dec tm pick_name) end
+
+fun append_decs tm = let
+  val tm = QCONV EVAL tm |> concl |> rand
+  val tms = fst (listSyntax.dest_list tm)
+  in (map append_dec tms; ()) end
+
+fun array_st () = get_ml_prog_state ()
+
+
+val _ = Define `
+  mk_binop name prim = Dlet (Pvar name)
+    (Fun "x" (Fun "y" (App prim [Var (Short "x"); Var (Short "y")])))`;
+
+val _ = Define `
+  mk_unop name prim = Dlet (Pvar name)
+    (Fun "x" (App prim [Var (Short "x")]))`;
+
+val _ = ml_prog_update (open_module "Array");
+
+
+val _ = append_decs
+   ``[Dtabbrev ["'a"] "array" (Tapp [Tvar "'a"] TC_array);
+      mk_binop "array" Aalloc;
+      mk_binop "sub" Asub;
+      mk_unop "length" Alength;
+      Dlet (Pvar "update")
+       (Fun "x" (Fun "y" (Fun "z"
+         (App Aupdate [Var (Short "x"); Var (Short "y"); Var (Short "z")])))) ]``
+
+
+val array_fromList = process_topdecs
+  `fun fromList l =
+    let val arr = Array.array (length l) 0
+      fun f l i =  
+        case l of
+          [] => arr
+        | h::t = (Array.update arr i h; f t (i + 1))
+    in f l 0 end`   
+
+val array_tabulate = process_topdecs
+  `fun tabulate n f =
+    let val arr = Array.array n 0
+      fun u x f =
+        case x of 
+          0 => arr
+        | (SUC x) => (Array.update arr x (f x); u x f)
+    in u n f end`
+
+(*val array_vector = process_topdecs
+  `fun vector arr =
+*)
+
+val _ = ml_prog_update (close_module NONE);
+
+fun prove_array_spec op_name =
+  xcf op_name (array_st()) \\ TRY xpull \\
+  fs [cf_aw8alloc_def, cf_aw8sub_def, cf_aw8length_def, cf_aw8update_def,
+      cf_aalloc_def, cf_asub_def, cf_alength_def, cf_aupdate_def] \\
+  irule local_elim \\ reduce_tac \\
+  fs [app_aw8alloc_def, app_aw8sub_def, app_aw8length_def, app_aw8update_def,
+      app_aalloc_def, app_asub_def, app_alength_def, app_aupdate_def] \\
+  xsimpl \\ fs [INT_def, NUM_def, WORD_def, w2w_def, UNIT_TYPE_def] \\
+  TRY (simp_tac (arith_ss ++ intSimps.INT_ARITH_ss) [])
+
+
+val array_alloc_spec = Q.store_thm ("array_alloc_spec",
+  `!n nv v.
+     NUM n nv ==>
+     app (p:'ffi ffi_proj) ^(fetch_v "Array.array" (array_st())) [nv; v]
+       emp (POSTv av. ARRAY av (REPLICATE n v))`,
+  prove_array_spec "Array.array");
+
+val array_sub_spec = Q.store_thm ("array_sub_spec",
+  `!a av n nv.
+     NUM n nv /\ n < LENGTH a ==>
+     app (p:'ffi ffi_proj) ^(fetch_v "Array.sub" (array_st())) [av; nv]
+       (ARRAY av a) (POSTv v. cond (v = EL n a) * ARRAY av a)`,
+  prove_array_spec "Array.sub");
+
+val array_length_spec = Q.store_thm ("array_length_spec",
+  `!a av.
+     app (p:'ffi ffi_proj) ^(fetch_v "Array.length" (array_st())) [av]
+       (ARRAY av a)
+       (POSTv v. cond (NUM (LENGTH a) v) * ARRAY av a)`,
+  prove_array_spec "Array.length");
+
+val array_update_spec = Q.store_thm ("array_update_spec",
+  `!a av n nv v.
+     NUM n nv /\ n < LENGTH a ==>
+     app (p:'ffi ffi_proj) ^(fetch_v "Array.update" (array_st()))
+       [av; nv; v]
+       (ARRAY av a)
+       (POSTv uv. cond (UNIT_TYPE () uv) * ARRAY av (LUPDATE v n a))`,
+  prove_array_spec "Array.update");
+
+val _ = export_theory ()
