basis/translation/mloptionProgScript.sml
@@ -1,13 +1,13 @@
-open preamble ml_translatorLib ml_progLib
+open preamble ml_translatorLib ml_progLib std_preludeTheory
      mloptionTheory
 
 (*this library depends on nothing *)
 val _ = new_theory"mloptionProg"
+
+val _ = translation_extends"std_prelude"
 val _ = ml_prog_update (open_module "Option");
 
 val _ = ml_prog_update (add_dec ``Dtabbrev ["'a"] "option" (Tapp [Tvar "'a"] (TC_name (Short "option")))`` I);
-
-val result = translate IS_SOME_DEF;
 
 val result = translate getOpt_def;
 
@@ -15,6 +15,11 @@ val result = translate IS_SOME_DEF;
 
 val result = next_ml_names := ["valOf"];
 val result = translate THE_DEF;
+val the_side_def = Q.prove(
+  `the_side = IS_SOME`,
+  FULL_SIMP_TAC std_ss [FUN_EQ_THM] THEN Cases
+  THEN FULL_SIMP_TAC (srw_ss()) [fetch "-" "the_side_def"])
+  |> update_precondition;
 
 val result = next_ml_names := ["join"];
 val result = translate OPTION_JOIN_DEF;
@@ -29,22 +34,9 @@ val result = translate compose_def;
 val result = translate composePartial_def;
 
 (*Functions declared in std_preludeLib *)
-val res = translate THE_DEF;
 val res = translate IS_NONE_DEF;
-val res = translate IS_SOME_DEF;
-val res = translate OPTION_MAP_DEF;
 val res = translate OPTION_MAP2_DEF;
 
-val the_side_def = Q.prove(
-  `the_side = IS_SOME`,
-  FULL_SIMP_TAC std_ss [FUN_EQ_THM] THEN Cases
-  THEN FULL_SIMP_TAC (srw_ss()) [fetch "-" "the_side_def"])
-  |> update_precondition;
-
-val option_map2_side_def = Q.prove(
-  `!f x y. option_map2_side f x y = T`,
-  FULL_SIMP_TAC (srw_ss()) [fetch "-" "option_map2_side_def",the_side_def])
-  |> update_precondition;
 
 
 
