translator/okasaki-examples/benchmarkScript.sml
@@ -1,12 +1,12 @@
 open HolKernel Parse boolLib bossLib;
-open bagTheory relationTheory bagLib miscTheory ml_translatorLib mini_preludeTheory;
+open bagTheory relationTheory bagLib miscTheory ml_translatorLib;
 open preamble
 
 val _ = new_theory "benchmark";
 
-open listTheory arithmeticTheory ml_translatorLib mini_preludeTheory;
+open listTheory arithmeticTheory ml_translatorLib mllistProgTheory;
 
-val _ = translation_extends "mini_prelude";
+val _ = translation_extends "mllistProg";
 
 (* copied from ImplicitQueueScript *)
 val _ = Hol_datatype `times = Once of 'a | Twice of times => times`;
